case_study/RiscvPmpBoundedInts/Sig.v
@@ -371,7 +371,7 @@ Module Export RiscvPmpSignature <: Signature RiscvPmpBase.
       | ptsto                    => [ty_xlenbits; ty_byte]
       | ptsto_readonly           => [ty_xlenbits; ty_byte]
       | encodes_instr            => [ty_word; ty_ast]
-      | ptstomem width           => [ty_xlenbits; ty.bvec (byte * width)]
+      | ptstomem width           => [ty_xlenbits; ty.bvec (width * byte)]
       | ptstoinstr               => [ty_xlenbits; ty_ast]
       end.
 
@@ -401,7 +401,7 @@ Module Export RiscvPmpSignature <: Signature RiscvPmpBase.
       | pmp_entries              => Some (MkPrecise ε [ty.list ty_pmpentry] eq_refl)
       | pmp_addr_access          => Some (MkPrecise ε [ty.list ty_pmpentry; ty_privilege] eq_refl)
       | pmp_addr_access_without  => Some (MkPrecise [ty_xlenbits] [ty.list ty_pmpentry; ty_privilege] eq_refl)
-      | ptstomem width           => Some (MkPrecise [ty_xlenbits] [ty.bvec (byte * width)] eq_refl)
+      | ptstomem width           => Some (MkPrecise [ty_xlenbits] [ty.bvec (width * byte)] eq_refl)
       | ptstoinstr               => Some (MkPrecise [ty_xlenbits] [ty_ast] eq_refl)
       | encodes_instr            => Some (MkPrecise [ty_word] [ty_ast] eq_refl)
       | _                        => None
